## quad

$
A_0 = \left[\begin{matrix}1 & 3 & 4 & 6\\3 & 2 & 3 & 0\\4 & 3 & 7 & 8\\6 & 0 & 8 & 10\end{matrix}\right]
$
<br>
$
T_1 = \left[\begin{matrix}1 & -3 & -4 & -6\\0 & 1 & 0 & 0\\0 & 0 & 1 & 0\\0 & 0 & 0 & 1\end{matrix}\right],
$
配平方项得
$
A_1 = T_1'A_0T_1 = \left[\begin{matrix}1 & 0 & 0 & 0\\0 & -7 & -9 & -18\\0 & -9 & -9 & -16\\0 & -18 & -16 & -26\end{matrix}\right]
$
<br>
$
T_2 = \left[\begin{matrix}1 & 0 & 0 & 0\\0 & 1 & - \frac{9}{7} & - \frac{18}{7}\\0 & 0 & 1 & 0\\0 & 0 & 0 & 1\end{matrix}\right],
$
配平方项得
$
A_2 = T_2'A_1T_2 = \left[\begin{matrix}1 & 0 & 0 & 0\\0 & -7 & 0 & 0\\0 & 0 & \frac{18}{7} & \frac{50}{7}\\0 & 0 & \frac{50}{7} & \frac{142}{7}\end{matrix}\right]
$
<br>
$
T_3 = \left[\begin{matrix}1 & 0 & 0 & 0\\0 & 1 & 0 & 0\\0 & 0 & 1 & - \frac{25}{9}\\0 & 0 & 0 & 1\end{matrix}\right],
$
配平方项得
$
A_3 = T_3'A_2T_3 = \left[\begin{matrix}1 & 0 & 0 & 0\\0 & -7 & 0 & 0\\0 & 0 & \frac{18}{7} & 0\\0 & 0 & 0 & \frac{4}{9}\end{matrix}\right]
$

## eigen

$
A = \begin{bmatrix}
        1 & 2 & 2 \\
        2 & 1 & 2 \\
        2 & 2 & 1
    \end{bmatrix}
$

$
|\lambda E - A| = 
\begin{vmatrix}
    \lambda - 1 & -2 & -2 \\
    -2 & \lambda - 1 & -2 \\
    -2 & -2 & \lambda - 1
\end{vmatrix} 
= (\lambda-5)(\lambda+1)^2
$

$
\lambda_1 = 5, \lambda_2 = -1
$

$
(\lambda_1 E - A)X = 
\begin{bmatrix}
    4 & -2 & -2 \\
    -2 & 4 & -2 \\
    -2 & -2 & 4
\end{bmatrix}
X = 0
$

$
X_1 = (1,1,1)^T
$

$
(\lambda_2 E - A)X = 
\begin{bmatrix}
    -2 & -2 & -2 \\
    -2 & -2 & -2 \\
    -2 & -2 & -2
\end{bmatrix}
X = 0
$

$
X_2 = (-1,1,0)^T, X_3 = (-1,0,1)^T
$
